Simulation & Adequacy, Part 1

theories/Semantics.v
@@ -1,18 +1,9 @@
-From Stdlib Require Import Utf8.
-
-From Stdlib Require Import Lists.List.
-From Stdlib Require Import ZArith.ZArith.
-
-From stdpp Require Import gmap.
-From stdpp Require Import relations.
-From stdpp Require Import tactics.
+From stdpp Require Import prelude.
 
 From RSL Require Import RTL.
-From RSL Require Import Logic.
 From RSL Require Import Notations.
 
 Import RTLNotations.
-Import ListNotations.
 
 (* Set Mangle Names. *)
 
@@ -41,8 +32,7 @@ Inductive pcstate : Type :=
     (args: list val) (* arguments to the call *)
 
 | ReturnState
-    (v: val) (* return value for the call *)
-.
+    (v: val). (* return value for the call *)
 
 Definition state : Type := list stackframe * pcstate * memory.
 
@@ -110,169 +100,6 @@ Notation "P '⊨' s '-{' n '}>' t" :=
 Variant final : state -> Prop :=
 | FinalState : ∀ v m, final ([], ReturnState v, m).
 
-Definition not_stuck (P: program) s := ∃ t, P ⊨ s ->> t.
+Definition can_progress (P: program) s := ∃ t, P ⊨ s ->> t.
 
-Definition stuck (P: program) s := ~(not_stuck P s) ∧ ~(final s).
-
-Lemma nsteps_inv_l {A : Type} {R : relation A} :
-  ∀ n x z, nsteps R (S n) x z → ∃ y : A, R x y ∧ nsteps R n y z.
-Proof. intros n x z H; inv H; eexists; eauto. Qed.
-
-Lemma ret_no_step P : ∀ v m t,
-  P ⊨ ([], ReturnState v, m) ->>* t ->
-  t = ([], ReturnState v, m).
-Proof.
-  intros v m t H.
-  destruct (rtc_inv _ _ H) as [-> | (y & Hstep & _)].
-  - easy.
-  - inv Hstep.
-Qed.
-
-Lemma ret_no_nsteps P : ∀ n v m t,
-  P ⊨ ([], ReturnState v, m) -{n}> t ->
-  t = ([], ReturnState v, m) ∧ n = 0.
-Proof.
-  intros [] v m t H.
-  - now inv H.
-  - destruct (nsteps_inv_l _ _ _ H) as (y & Hstep & _).
-    inv Hstep.
-Qed.
-
-Lemma lift_step P : ∀ σ s m σ' t m' Σ,
-  P ⊨ (σ, s, m) ->> (σ', t, m') ->
-  P ⊨ (σ ++ Σ, s, m) ->> (σ' ++ Σ, t, m').
-Proof.
-  intros ? ? ? ? ? ? ? H; inv H; econstructor; now eauto.
-Qed.
-
-Lemma unlift_step P : ∀ σ s m σ' t m' Σ,
-  P ⊨ (σ ++ Σ, s, m) ->> (σ' ++ Σ, t, m') ->
-  P ⊨ (σ, s, m) ->> (σ', t, m').
-Proof.
-  intros ? ? ? ? ? ? ? H; inv H;
-    rewrite ? app_comm_cons in *;
-    eassert _ by (eapply app_inv_tail; eassumption);
-    subst; econstructor; now eauto.
-Qed.
-
-Theorem lift_steps P : ∀ σ s m σ' t m' Σ,
-  P ⊨ (σ, s, m) ->>* (σ', t, m') ->
-  P ⊨ (σ ++ Σ, s, m) ->>* (σ' ++ Σ, t, m').
-Proof.
-  intros σ s m σ' t m' Σ Hrtc.
-  remember (σ, s, m) as x eqn:Hx.
-  remember (σ', t, m') as y eqn:Hy.
-  induction Hrtc as [ y | x y z H Hrtc IH]
-    in σ, s, m, Hx, σ', t, m', Hy |- *.
-  - subst. inv Hy. reflexivity.
-  - subst. destruct y as [[] ?].
-    etransitivity.
-    + apply rtc_once. apply lift_step. eassumption.
-    + eauto.
-Qed.
-
-Lemma ret_not_stuck : ∀ P frame σ v m,
-  not_stuck P (frame :: σ, ReturnState v, m).
-Proof. intros P []. repeat econstructor; now eauto. Qed.
-
-Lemma ret_stuck_in_empty : ∀ P v m,
-  ~ not_stuck P ([], ReturnState v, m).
-Proof. intros P v m [u H]. inv H. Qed.
-
-Lemma lift_not_stuck : ∀ P σ Σ s m,
-  not_stuck P (σ, s, m) ->
-  not_stuck P (σ ++ Σ, s, m).
-Proof. intros P σ Σ s m [[[] ?] Ht]. eexists. apply lift_step. eassumption. Qed.
-
-Lemma unfold_call P fn : ∀ n res f pc ρ args m σ t m',
-  P ⊨ ([Stackframe res f pc ρ], CallState fn args, m) -{n}> (σ, t, m') ->
-  (∃ σ',
-      σ = σ' ++ [Stackframe res f pc ρ]
-      ∧ P ⊨ ([], CallState fn args, m) -{n}> (σ', t, m'))
-  ∨
-    (∃ m1 m2 v m'',
-        n = 1 + m1 + m2
-        ∧ P ⊨ ([], CallState fn args, m) -{m1}> ([], ReturnState v, m'')
-        ∧ P ⊨ ([], State f pc (set_reg res v ρ), m'') -{m2}> (σ, t, m')
-    ).
-Proof.
-  intros n.
-  induction n as [ | n IH ];
-    intros res f pc ρ args m σ t m' Hrtc.
-  - inv Hrtc. left. exists []. split; auto. constructor.
-  - apply nsteps_inv_r in Hrtc. destruct Hrtc as ([[] ?] & Hrtc & Hstep).
-    apply IH in Hrtc.
-    destruct Hrtc
-      as [(σ' & -> & Hlift) | (m1 & m2 & v & m'' & Hn & Hcall & Hrest)].
-    + inv Hstep as [ | | | | | | | | ? ? ? ? ? ? v ? ? Hσ];
-        try (left; eexists; split;
-             [ rewrite ? app_comm_cons; reflexivity
-             | eapply nsteps_r; [ now apply Hlift | econstructor; now eauto]
-             ]
-          ).
-      destruct σ'; inv Hσ.
-      * right. exists n, 0, v, m'. repeat split; eauto. constructor.
-      * left. eexists. split.
-        -- reflexivity.
-        -- eapply nsteps_r; [ now apply Hlift | econstructor; now eauto].
-    + inversion Hstep; subst; right; (exists m1, (S m2), v, m''); repeat split;
-        now eauto || (eapply nsteps_r;
-                      [ now apply Hrest | econstructor; now eauto]).
-Qed.
-
-Lemma get_regs_insert : ∀ regs r v ρ,
-  r ∉ regs ->
-  get_regs regs (<[r := v]> ρ) = get_regs regs ρ.
-Proof.
-  intros regs r v ρ.
-  induction regs as [|r' regs' IH]; intros Hnotin; [reflexivity |].
-  simpl. f_equal.
-  - unfold get_reg. rewrite (lookup_insert_ne ρ); set_solver.
-  - apply IH. set_solver.
-Qed.
-
-Lemma get_regs_init_regs : ∀ regs args,
-  NoDup regs ->
-  length args = length regs ->
-  get_regs regs (init_regs args regs) = args.
-Proof.
-  intros regs args Hnodup.
-  revert args.
-  induction Hnodup as [|r regs Hnotin Hnodup IH]; intros args Hlen.
-  - destruct args; [reflexivity | discriminate Hlen].
-  - destruct args as [|v args]; [discriminate Hlen |].
-    simpl in Hlen. injection Hlen as Hlen'.
-    simpl. f_equal.
-    + unfold get_reg. now rewrite (lookup_insert_eq (init_regs args regs)).
-    + rewrite get_regs_insert by exact Hnotin.
-      apply IH. exact Hlen'.
-Qed.
-
-Lemma get_reg_set_reg_eq : ∀ r v ρ,
-  get_reg r (set_reg r v ρ) = v.
-Proof.
-  intros r v ρ.
-  unfold get_reg, set_reg.
-  now rewrite (lookup_insert_eq ρ).
-Qed.
-
-Lemma get_reg_set_reg_neq : ∀ r r' v ρ,
-  r ≠ r' -> get_reg r (set_reg r' v ρ) = get_reg r ρ.
-Proof.
-  intros r r' v ρ Hneq.
-  unfold get_reg, set_reg.
-  now rewrite (lookup_insert_ne ρ).
-Qed.
-
-Tactic Notation "simpl_reg" "by" tactic3(tac) :=
-  repeat match goal with
-    | _ => progress tac
-    | |- context[get_reg _ (set_reg _ _ _)] =>
-        (rewrite get_reg_set_reg_neq by tac)
-        || (rewrite get_reg_set_reg_eq by tac)
-    | H: get_reg ?r ?rho = _ |- context[get_reg ?r ?rho] =>
-        repeat rewrite H
-    end.
-
-Tactic Notation "simpl_reg" :=
-  simpl_reg by repeat (f_equal || lia || unfold_Prop || split).
+Definition stuck (P: program) s := ~(can_progress P s) ∧ ~(final s).
