theories/Sim.v
@@ -1,135 +1,75 @@
-From Stdlib Require Import Utf8.
-
-From Stdlib Require Import Lists.List.
-From Stdlib Require Import Strings.String.
-From Stdlib Require Import ZArith.ZArith.
-From Stdlib Require Import Lia.
-
-From stdpp Require Import relations.
+From stdpp Require Import prelude.
 From stdpp Require Import tactics.
 
-From RSL Require Import RTL.
-From RSL Require Import Notations.
-From RSL Require Import Semantics.
-From RSL Require Import Logic.
-From RSL Require Import WP.
+From Coinduction Require Import all.
 
-Import RTLNotations.
-Import ListNotations.
+From RSL Require Import RTL.
+From RSL Require Import Semantics.
+From RSL Require Import SemanticsSpec.
+From RSL Require Import Refinement.
+
+(* Set Mangle Names. *)
 
 Section Sim.
-  Variable P: program.
+  Context (stepₜ stepₛ: state -> state -> Prop).
 
-  Definition exec : Type := nat → state.
+  Context (Φ: observation).
 
-  (** Asserts that f is a diverging execution from s. *)
-  Definition diverging_execution (f: exec) (s: state) :=
-    f 0 = s ∧ ∀ n, P ⊨ f n ->> f (S n).
+  Variant final : state -> state -> Prop :=
+  | FinalState : ∀ vₜ mₜ vₛ mₛ,
+    Φ (vₜ, mₜ) (vₛ, mₛ) ->
+    final ([], ReturnState vₜ, mₜ) ([], ReturnState vₛ, mₛ).
 
-  (** s is a diverging state if s is the begining of some diverging execution *)
-  Definition diverges (s: state) := ∃ f, diverging_execution f s.
+  Inductive sim_lfp' (gfp: state -> state -> Prop) : state ->  state -> Prop :=
+  | BothFinal : ∀ t s,
+    final t s -> sim_lfp' gfp t s
 
-  Variant behavior :=
-  | Terminating (v: val) (m: memory)
-  | Diverging
-  | Unknown.
+  | SourceStuck : ∀ t s,
+    stuck P s -> sim_lfp' gfp t s
 
-  Inductive behavior_order : behavior -> behavior -> Prop :=
-  | TerminatingOrder : ∀ v m, behavior_order (Terminating v m) (Terminating v m)
-  | DivergingOrder : behavior_order Diverging Diverging
-  | UnkownOrder : ∀ s, behavior_order s Unknown.
+  | TargetStutter : ∀ t s s',
+    P ⊨ s ->> s' -> sim_lfp' gfp t s' -> sim_lfp' gfp t s
 
-  Instance behavior_order_inst : PartialOrder behavior_order.
+  | TargetSteps : ∀ t s,
+    can_progress P t ->
+    (∀ t', P ⊨ t ->> t' -> sim_lfp' gfp t' s) ->
+    sim_lfp' gfp t s
+
+  | BothSteps : ∀ t s,
+    can_progress P t ->
+    (∀ t', P ⊨ t ->> t' -> ∃ s', P ⊨ s ->> s' ∧ gfp t' s') ->
+    sim_lfp' gfp t s.
+
+  Instance sim_lfp'_proper : Proper (leq ==> leq) sim_lfp'.
   Proof.
-    split. 1: split.
-    - intros []; constructor.
-    - intros x y z Hxy Hyz. inv Hxy.
-      + assumption.
-      + assumption.
-      + inv Hyz. constructor.
-    - intros x y Hxy Hyx. inv Hxy; try reflexivity.
-      now inv Hyx.
-  Qed.
-  Instance behavior_order_notation : SqSubsetEq behavior := behavior_order.
-
-  (* [beh s] is the set of all the behaviors of [s] *)
-  Inductive beh : state -> behavior -> Prop :=
-  | IsTerminating : ∀ v m,
-      beh ([], ReturnState v, m) (Terminating v m)
-  | IsDiverging : ∀ s,
-      diverges s ->
-      beh s Diverging
-  | IsStuck : ∀ s,
-      stuck P s ->
-      beh s Unknown
-  | IsSteping : ∀ s t b,
-      beh t b ->
-      P ⊨ s ->> t ->
-      beh s b.
-
-  Instance beh_elem_state : ElemOf behavior (behavior -> Prop) := fun b P => P b.
-
-  (* [s] is terminating iff there is a execution from [s] to a final state. *)
-  Lemma has_terminating_behavior : ∀ s v m,
-    Terminating v m ∈ beh s <-> P ⊨ s ->>* ([], ReturnState v, m).
-  Proof.
-    intros s v m. split; intros H.
-    - remember (Terminating v m) as b eqn:Hb.
-      induction H as [ | | | s t b ? IH Hstep ] in s, H, v, m, b, Hb |- *; inv Hb.
-      + constructor.
-      + apply rtc_l with t; now auto.
-    - remember ([], ReturnState v, m) as t eqn:Ht.
-      induction H as [ | s t u Hstep Hrtc IH ]
-        in t, Ht, v, m, H |- *; subst.
-      + constructor.
-      + econstructor. 2: eassumption. firstorder.
+    intros gfp gfp' Hgfp s t H. induction H as [ | | | | ? ? ? H ];
+      try (econstructor; eassumption || now apply Hlfp).
+    apply BothSteps; eauto. intros t' Hstep.
+    destruct (H _ Hstep) as (? & ? & ?).
+    eexists. split; eassumption || now apply Hgfp.
   Qed.
 
-  (* [s] is diverging iff [s] has a diverging execution *)
-  Lemma has_diverging_behavior : ∀ s,
-    Diverging ∈ beh s <-> diverges s.
+  Definition sim_lfp : mon (state -> state -> Prop) := {| body := sim_lfp' |}.
+
+  Definition sim := gfp sim_lfp.
+
+  Lemma sim_coind (R : state -> state -> Prop) :
+    (∀ t s, R t s -> sim_lfp R t s) ->
+    ∀ t s, R t s -> sim t s.
   Proof.
-    intros s. split; intros H.
-    - remember Diverging as b eqn:Hb.
-      induction H as [ | | | s t b ? IH Hstep ]
-        in s, b, Hb, H |- *; try discriminate Hb; eauto.
-      destruct (IH Hb) as (f & Hinit & Hsucc).
-      exists (fun n => match n with O => s | S n => f n end). split.
-      + reflexivity.
-      + intros []; now subst.
-    - now constructor.
+    intros Hstep. unfold sim.
+    coinduction Re cih. intros t s HR.
+    assert (HRe: R <= elem Re). {
+      intros t' s' HR'. now apply cih.
+    }
+    apply (sim_lfp'_proper R _ HRe).
+    now apply Hstep.
   Qed.
 
-  (* [s] has a unknown behavior if [s] reduces to a stuck state. *)
-  Lemma has_stuck_behavior : ∀ s,
-    Unknown ∈ beh s <-> ∃ t, P ⊨ s ->>* t ∧ stuck P t.
+  Lemma sim_stuck_example t s :
+    stuck P t -> stuck P s -> sim t s.
   Proof.
-    intros s. split; intros H.
-    - remember Unknown as b eqn:Hb.
-      induction H as [ s | | | s t b ? IH Hstep ]
-        in s, b, Hb, H |- *; try discriminate Hb; eauto.
-      + exists s. now split.
-      + destruct (IH Hb) as (u & Hrtc & Hstuck).
-        exists u. split.
-        * now apply rtc_l with t.
-        * assumption.
-    - destruct H as (u & Hrtc & Hstuck).
-      induction Hrtc  as [ | s t u Hstep Hrtc IH] in s, u, Hrtc, Hstuck |- *.
-      + now constructor.
-      + eapply IsSteping.
-        * now apply IH.
-        * easy.
+    intros Ht Hs. unfold sim.
+    step. apply BothStuck. all: assumption.
   Qed.
-
-  (* A definition of state refinement:
-     - if the target terminates on (v, m),
-       the source must either terminate on (v, m) or be stuck.
-     - if the target diverges,
-       the source must either diverges or be stuck.
-     - if the target is stuck, the source should also be stuck.
-   *)
-  Definition refines (t: state) (s: state) :=
-    ∀ b, b ∈ beh t -> ∃ b', b' ∈ beh s ∧ b ⊑ b'.
-
-
 End Sim.
