theories/Adequacy.v
@@ -1,0 +1,67 @@
+From stdpp Require Import prelude.
+
+From Coinduction Require Import all.
+
+From RSL Require Import RTL.
+From RSL Require Import Semantics.
+From RSL Require Import SemanticsSpec.
+From RSL Require Import Refinement.
+From RSL Require Import Sim.
+
+Section Adequacy.
+  Context (P: program).
+  Context {Φ: observation} `{!PreOrder Φ}.
+
+  Notation "t '≲' s '{{' Φ '}}'" := (gfp (sim_lfp P Φ) t s).
+
+  Local Instance beh_elem : ElemOf behavior state := λ b s, beh P s b.
+  Local Instance beh_subset_eq : SqSubsetEq behavior := @behavior_order Φ.
+
+  Lemma sim_unroll t s :
+    t ≲ s {{ Φ }} -> sim_lfp' P Φ (gfp (sim_lfp P Φ)) t s.
+  Proof.
+    intros H. now apply (gfp_pfp (sim_lfp _ _)).
+  Qed.
+
+  Lemma converging_sim : ∀ (t s: state) v m,
+    t ≲ s {{ Φ }} ->
+    Terminating v m ∈ t ->
+    ∃ b, b ∈ s ∧ Terminating v m ⊑ b.
+  Proof.
+    intros t s v m Hsim Hb.
+    erewrite -> (@has_terminating_behavior P) in Hb by eassumption.
+    destruct Hb as (t' & Hrtc & Hfin).
+    pose proof (final_to_final _ _ _ Hfin) as Hf.
+    revert s Hsim.
+    induction Hrtc as [ t' | t t' t'' Hstep Hrtc IH ].
+    - intros s Hsim.
+      apply sim_unroll in Hsim.
+      induction Hsim; subst.
+      + inv H. inv Hfin. exists vₛ, mₛ. now repeat constructor.
+      + exfalso. eapply final_not_stuck; eassumption.
+      + destruct (IHHsim Hfin Hf) as (v' & m' & Ht' & HΦ).
+        eexists. eexists. split.
+        * eapply IsSteping. apply Ht'. assumption.
+        * apply HΦ.
+      + exfalso. eapply final_no_progress; eassumption.
+      + exfalso. eapply final_no_progress; eassumption.
+    - intros s Hsim.
+      apply sim_unroll in Hsim.
+      induction Hsim; subst.
+      + inv H. inv Hstep.
+      + exfalso. destruct H as [Hs _].
+        apply Hs. eexists. eassumption.
+      + destruct (IHHsim Hstep) as (v' & m' & Hs' & HΦ).
+        eexists. eexists. split.
+        * eapply IsSteping. apply Hs'. assumption.
+        * apply HΦ.
+      + apply (IH Hfin Hf).
+        step.
+        apply H0. assumption.
+      + destruct (H0 _ Hstep) as (s' & Hs' & HΦ).
+        apply (IH Hfin Hf) in HΦ. destruct HΦ as (v' & m' & Hterm & HΦ).
+        eexists. eexists. split.
+        * eapply IsSteping; eauto.
+        * apply HΦ.
+  Qed.
+End Adequacy.
