theories/Commons/Language.v
@@ -1,0 +1,48 @@
+From stdpp Require Import prelude.
+
+Section language_mixin.
+  Context {state value : Type}.
+
+  Context (step : state -> state -> Prop).
+
+  Context (can_progress : state -> Prop).
+  Context (is_final : state -> option value).
+
+  Record LanguageMixin := {
+      mixin_final_no_progress : ∀ s v, is_final s = Some v -> can_progress s -> False;
+      mixin_can_progress_must_step : ∀ s, can_progress s -> ∃ t, step s t;
+    }.
+End language_mixin.
+
+Structure language :=
+  Language {
+      state : Type;
+      value : Type;
+
+      step : state -> state -> Prop;
+
+      can_progress : state -> Prop;
+      is_final : state -> option value;
+
+      language_mixin : LanguageMixin step can_progress is_final;
+    }.
+
+Arguments step {_} _ _.
+Arguments can_progress {_} _.
+Arguments is_final {_}.
+
+Section Language.
+  Context {Λ: language}.
+
+  Definition stuck (s : state Λ) : Prop :=
+    is_final s = None ∧ ~ can_progress s.
+
+  Lemma final_not_stuck : ∀ s v,
+    is_final s = Some v -> ~ stuck s.
+  Proof. intros ? ? H [? ?]. inv H. Qed.
+
+  Lemma progress_not_stuck : ∀ s,
+    can_progress s -> ~ stuck s.
+  Proof. intros ? ? []. tauto. Qed.
+
+End Language.
