theories/Logic.v
@@ -1,4 +1,4 @@
-From Stdlib Require Import Utf8.
+From stdpp Require Import base.
 
 From RSL Require Import RTL.
 
