theories/Refinement.v
@@ -1,0 +1,140 @@
+From stdpp Require Import prelude.
+
+From Coinduction Require Import all.
+
+From RSL.Commons Require Import Language.
+
+(* Set Mangle Names. *)
+
+Section Refinement.
+  Context {Λ: language}.
+
+  Definition observation : Type := value Λ -> value Λ -> Prop.
+
+  Context {Obs: observation} `{!PreOrder Obs}.
+
+  Program Definition diverges_: mon (state Λ -> Prop) :=
+    {| body R s := ∃ s', step s s' ∧ R s' |}.
+  Next Obligation. firstorder. Qed.
+
+  Definition diverges : state Λ -> Prop := gfp diverges_.
+
+  Lemma diveges_sound : ∀ f,
+    (∀ n, step (f n) (f (S n))) -> diverges (f 0).
+  Proof.
+    intros f Hf. cut (∀ n, diverges (f n)); auto.
+    unfold diverges. coinduction R cih.
+    intros n. exists (f (S n)); auto.
+  Qed.
+
+  Variant behavior :=
+  | Terminating (v: value Λ)
+  | Diverging
+  | Unknown.
+
+  Inductive behavior_order : behavior -> behavior -> Prop :=
+  | TerminatingOrder : ∀ vₜ vₛ,
+    Obs vₜ vₛ -> behavior_order (Terminating vₜ) (Terminating vₛ)
+  | DivergingOrder : behavior_order Diverging Diverging
+  | UnkownOrder : ∀ s, behavior_order s Unknown.
+
+  Instance beh_pre_order : PreOrder behavior_order.
+  Proof.
+    split.
+    - intros []; now constructor.
+    - intros x y z Hxy Hyz. inv Hxy; inv Hyz; constructor.
+      etransitivity; eassumption.
+  Qed.
+
+  Instance behavior_order_notation : SqSubsetEq behavior := behavior_order.
+
+  (* [beh s] is the set of all the behaviors of [s] *)
+  Inductive beh : state Λ -> behavior -> Prop :=
+  | IsTerminating : ∀ s v,
+      is_final s = Some v ->
+      beh s (Terminating v)
+  | IsDiverging : ∀ s,
+      diverges s ->
+      beh s Diverging
+  | IsStuck : ∀ s,
+      stuck s ->
+      beh s Unknown
+  | IsSteping : ∀ s t b,
+      beh t b ->
+      step s t ->
+      beh s b.
+
+  Instance beh_elem_state : ElemOf behavior (state Λ) := λ b s, beh s b.
+
+  (* [s] is terminating iff there is a execution from [s] to a final state. *)
+  Lemma has_terminating_behavior : ∀ s v,
+    Terminating v ∈ s <-> ∃ t, rtc step s t ∧ is_final t = Some v.
+  Proof.
+    intros s v. split; intros Hbeh.
+    - remember (Terminating v) as b eqn:Hb.
+      induction Hbeh as [ s | | | s t b ? IH Hstep ]; inv Hb; auto.
+      + exists s. now constructor.
+      + destruct (IH eq_refl) as (t' & Hrtc & Hfin). clear IH.
+        exists t'. split; eauto. now apply rtc_l with t.
+    - destruct Hbeh as (t & Hrtc & Hfin).
+      induction Hrtc as [ | s t u Hstep Hrtc IH ].
+      + now constructor.
+      + eapply IsSteping; eauto. now apply IH.
+  Qed.
+
+  (* [s] is diverging iff [s] has a diverging execution *)
+  Lemma has_diverging_behavior : ∀ s,
+    Diverging ∈ s <-> diverges s.
+  Proof.
+    intros s. split; intros Hbeh.
+    - revert s Hbeh. unfold diverges. coinduction R cih.
+      intros s Hbeh. inv Hbeh.
+      + apply (gfp_pfp diverges_) in H.
+        destruct H as (s' & Hstep & Hdiv).
+        exists s'. split; auto. apply cih. apply IsDiverging. assumption.
+      + exists t. split; auto.
+    - now apply IsDiverging.
+  Qed.
+
+  (* [s] has a unknown behavior if [s] reduces to a stuck state. *)
+  Lemma has_stuck_behavior : ∀ s,
+    Unknown ∈ s <-> ∃ t, rtc step s t ∧ stuck t.
+  Proof.
+    intros s. split; intros Hbeh.
+    - remember Unknown as b eqn:Hb.
+      induction Hbeh as [ | | s | s t b ? IH Hstep ]; inv Hb; auto.
+      + exists s. now split.
+      + destruct (IH eq_refl) as (u & Hrtc & Hstuck).
+        exists u. split.
+        * now apply rtc_l with t.
+        * assumption.
+    - destruct Hbeh as (u & Hrtc & Hstuck).
+      induction Hrtc  as [ | s t u Hstep Hrtc IH].
+      + now constructor.
+      + eapply IsSteping.
+        * now apply IH.
+        * easy.
+  Qed.
+End Refinement.
+
+(* A definition of state refinement:
+   - if the target terminates on (v, m),
+   the source must either terminate on (v, m) or be stuck.
+   - if the target diverges,
+   the source must either diverges or be stuck.
+   - if the target is stuck, the source should also be stuck.
+ *)
+(* Definition refines (t: state Λ) (s: state Λ) := *)
+(*   ∀ b, b ∈ t -> ∃ b', b' ∈ s ∧ b ⊑ b'. *)
+
+(* Instance refines_preorder : PreOrder refines. *)
+(* Proof. *)
+(*   split. *)
+(*   - intros s b Hb. exists b. now split. *)
+(*   - intros s t u Hst Htu b Hb. *)
+(*     destruct (Hst _ Hb) as (b' & Hb' & ?). *)
+(*     destruct (Htu _ Hb') as (b'' & Hb'' & ?). *)
+(*     exists b''. split. *)
+(*       + assumption. *)
+(*       + etransitivity; eassumption. *)
+(* Qed. *)
